Fixed and discharged the unprovable injectivity and caseConsistent assumptions for anf correctness.
convert_env always produces an injective conId_map, one doesn't need default_tag reasoning,
the caseConsistent assumption is replaced by a coherence assumption between the tag map and the constructor environment.

Also add a correctness file linking MetaRocq's pipeline and the ANF translation.
ANF relies on a slightly stronger condition of wellformedness than what is provided by MetaRocq

This formalizes the remaining mismatch between metarocq's pipeline and certirocq's LambdaANF:

- primitives are not supported in fuel_sem, and primitive arrays are forbidden in ANF conversion.
- the environment must be axiom free, as usual.

Prove that all constructors in the environment are properly registered in the tag map

Change case_consistent to coherence between tgm and cenv

correctness proof

WIP connecting to CertiRocq

Fill the values in the environment precondition for CertiRocq's toplevel theorem

WIP in correctness proof

al

Cleanup the correctness proof linking metarocq's pipeline with anf conversion

Update nix toolbox/action

WIP trying to prove coherence

convert_env always produces coherent tag maps and constructor environments

We store the inductive tag along the constructor tag in the tag map, facilitating proofs of coherence with the constructor environment.

Discharges the last remaining assumption of convert_top_anf_correct

Fill remaining admits in anf_corresp

Move proofs about convert_env to a separate module

Moved convert_env proofs to a separate module, cleaned-up correctness

Add a lemma showing totality of anf translation for well-formed terms

Update plugin manifest, fixing plugin compilation

Use inj_conIdMap def everywhere

theories/LambdaBox_to_LambdaANF/anf_toplevel.v
@@ -15,7 +15,7 @@ From CertiRocq.LambdaANF Require Import
   tactics identifiers bounds term_util rename set_util stemctx.
 From MetaRocq.Utils Require Import All_Forall.
 From CertiRocq.LambdaBox_to_LambdaANF Require Import
-  common anf fuel_sem wf anf_corresp anf_util anf_correct anf_global
+  common anf fuel_sem wf anf_corresp anf_util anf_convert_env anf_correct anf_global
   anf_divergence.
 
 Import ListNotations.
@@ -33,11 +33,9 @@ Section Refinement.
   Context {efl : EEnvFlags}.
   Context (HnoAxioms : has_axioms = false).
 
-  Context (dcon_to_tag_inj :
-    forall dc dc',
-      dcon_to_tag default_tag dc tgm = dcon_to_tag default_tag dc' tgm -> dc = dc').
-
-  Context (cenv_case_consistent : forall P ctag, caseConsistent cenv P ctag).
+  Context (dcon_to_tag_inj : inj_conIdMap tgm).
+  Context (Htgm : registered_constructors tgm Σ).
+  Context (cenv_tgm_coh : cenv_tgm_coherence cenv tgm).
 
   Let Hf_src := LambdaBox_resource_fuel.
   Let Ht_src := LambdaBox_resource_trace.
@@ -110,7 +108,7 @@ Section Refinement.
     in
     match v1, v2 with
     | fuel_sem.Con_v c1 vs1, Vconstr c2 vs2 =>
-      dcon_to_tag default_tag c1 tgm = c2 /\ Forall2_aux vs1 vs2
+      dcon_to_tag c1 tgm = Some c2 /\ Forall2_aux vs1 vs2
     | fuel_sem.Clos_v _ _ _, Vfun _ _ _ => True
     | fuel_sem.ClosFix_v _ _ _, Vfun _ _ _ => True
     | _, _ => False
@@ -119,7 +117,7 @@ Section Refinement.
   Definition value_ref (v1 : fuel_sem.value) (v2 : val) : Prop :=
     match v1, v2 with
     | fuel_sem.Con_v c1 vs1, Vconstr c2 vs2 =>
-      dcon_to_tag default_tag c1 tgm = c2 /\ Forall2 value_ref' vs1 vs2
+      dcon_to_tag c1 tgm = Some c2 /\ Forall2 value_ref' vs1 vs2
     | fuel_sem.Clos_v _ _ _, Vfun _ _ _ => True
     | fuel_sem.ClosFix_v _ _ _, Vfun _ _ _ => True
     | _, _ => False
@@ -167,7 +165,7 @@ Section Refinement.
     induction v1 using fuel_sem.value_ind'; intros v2 v3 Hval Hpre; inv Hval.
     - rewrite preord_val_eq in Hpre.
       destruct v3; try contradiction. inv Hpre.
-      simpl. split. reflexivity.
+      simpl. split. assumption.
 
       revert l vs' H2 H1.
       induction H; intros.
@@ -213,13 +211,13 @@ Section Refinement.
         _ Σ nat Hf_src Ht_src
         Hglob_term Hwf_glob
         HnoVar HnoEvar HnoCoFix HnoLazy Hblocks HnoArray
-        no_prims Hcmap_complete Hcmap_sound Hcmap_nodup_keys Hcmap_eval_coherent).
+        no_prims Hcmap_complete Hcmap_sound Hcmap_nodup_keys Hcmap_eval_coherent Htgm).
     destruct (@global_ctx_correct_top
                 func_tag kon_tag default_tag default_itag
                 tgm cmap cenv Σ efl
                 HnoAxioms
-                dcon_to_tag_inj
-                cenv_case_consistent
+                dcon_to_tag_inj Htgm
+                cenv_tgm_coh
                 Hglob_term Hglob_fuel_zero Hglob_wf
                 prim_map prims Hwf_glob
                 HnoVar HnoEvar HnoCoFix HnoLazy Hblocks HnoArray
@@ -233,8 +231,8 @@ Section Refinement.
     pose proof (@anf_cvt_correct
                   func_tag default_tag default_itag
                   tgm cmap cenv Σ efl
-                  dcon_to_tag_inj
-                  cenv_case_consistent Hcmap_eval_coherent
+                  dcon_to_tag_inj 
+                  cenv_tgm_coh Hcmap_eval_coherent
                   Hglob_term Hglob_fuel_zero Hglob_wf val_rel_exists
                   [] e (Val src_v) f t Heval)
       as Hcorr.
@@ -391,13 +389,13 @@ Section Refinement.
         _ Σ nat Hf_src Ht_src
         Hglob_term Hwf_glob
         HnoVar HnoEvar HnoCoFix HnoLazy Hblocks HnoArray
-        no_prims Hcmap_complete Hcmap_sound Hcmap_nodup_keys Hcmap_eval_coherent).
+        no_prims Hcmap_complete Hcmap_sound Hcmap_nodup_keys Hcmap_eval_coherent Htgm).
     destruct (@global_ctx_correct_top
                 func_tag kon_tag default_tag default_itag
                 tgm cmap cenv Σ efl
                 HnoAxioms
-                dcon_to_tag_inj              
-                cenv_case_consistent
+                dcon_to_tag_inj Htgm         
+                cenv_tgm_coh
                 Hglob_term Hglob_fuel_zero Hglob_wf
                 prim_map prims Hwf_glob
                 HnoVar HnoEvar HnoCoFix HnoLazy Hblocks HnoArray
@@ -443,7 +441,7 @@ Section Refinement.
                     func_tag default_tag default_itag
                     tgm cmap cenv Σ efl
                     dcon_to_tag_inj                    
-                    cenv_case_consistent Hcmap_eval_coherent
+                    cenv_tgm_coh Hcmap_eval_coherent
                     Hglob_term Hglob_fuel_zero Hglob_wf val_rel_exists
                     [] e cin t Hoot)
         as Hcorr_oot.
@@ -526,10 +524,8 @@ Section ComputationalRefinement.
   Context {efl : EEnvFlags}.
   Context (HnoAxioms : has_axioms = false).
 
-  Context (dcon_to_tag_inj :
-    forall dc dc',
-      dcon_to_tag default_tag dc tgm = dcon_to_tag default_tag dc' tgm -> dc = dc').
-
+  Context (dcon_to_tag_inj : inj_conIdMap tgm).
+  Context (Htgm : registered_constructors tgm Σ).
   Context (Hglob_term :
     forall k decl body,
       declared_constant Σ k decl ->
@@ -571,11 +567,10 @@ Section ComputationalRefinement.
     end.
 
   Definition refines_top (ie : ienv) (M : nat) (e_src : EAst.term) (e_tgt : exp) : Prop :=
-    refines default_tag tgm (top_cenv ie) Σ M e_src e_tgt.
+    refines tgm (top_cenv ie) Σ M e_src e_tgt.
 
   Context (ie : ienv).
-  Context (cenv_case_consistent_top :
-    forall P ctag, caseConsistent (top_cenv ie) P ctag).
+  Context (cenv_tgm_coh : cenv_tgm_coherence (top_cenv ie) tgm).
 
   Theorem convert_top_anf_correct next_id e e_tgt comp_d' :
     wellformed Σ 0 e = true ->
@@ -590,15 +585,15 @@ Section ComputationalRefinement.
                  tgm Σ efl HnoAxioms
                  prim_map prims Hwf_glob
                  HnoVar HnoEvar HnoCoFix HnoLazy Hblocks HnoArray
-                 no_prims
+                 no_prims Htgm
                  next_id ie e e_tgt comp_d' Hwf Hrun)
       as [cm [Sg' [S' [C_env [C [r [Hglob_cvt [Hmain_cvt ->]]]]]]]].
     eapply (@anf_correct_top_explicit
               func_tag kon_tag default_tag default_itag
               tgm cm (top_cenv ie) Σ efl
               HnoAxioms
-              dcon_to_tag_inj              
-              cenv_case_consistent_top
+              dcon_to_tag_inj Htgm             
+              cenv_tgm_coh
               Hglob_term Hglob_fuel_zero Hglob_wf
               prim_map prims Hwf_glob
               HnoVar HnoEvar HnoCoFix HnoLazy Hblocks HnoArray
@@ -624,15 +619,15 @@ Section ComputationalRefinement.
                  tgm Σ efl HnoAxioms
                  prim_map prims Hwf_glob
                  HnoVar HnoEvar HnoCoFix HnoLazy Hblocks HnoArray
-                 no_prims
+                 no_prims Htgm
                  next_id ie e e_tgt comp_d' Hwf Hrun)
       as [cm [Sg' [S' [C_env [C [r [Hglob_cvt [Hmain_cvt ->]]]]]]]].
     eapply (@anf_divergence_top_explicit
               func_tag kon_tag default_tag default_itag
               tgm cm (top_cenv ie) Σ efl
               HnoAxioms
-              dcon_to_tag_inj
-              cenv_case_consistent_top
+              dcon_to_tag_inj Htgm
+              cenv_tgm_coh
               Hglob_term Hglob_fuel_zero Hglob_wf
               prim_map prims Hwf_glob
               HnoVar HnoEvar HnoCoFix HnoLazy Hblocks HnoArray
