theories/Compiler/correctness.v
@@ -1,0 +1,284 @@
+From Stdlib Require Import ssreflect ssrbool.
+From Equations Require Import Equations.
+
+Require Export LambdaANF.toplevel Codegen.toplevel CodegenWasm.toplevel.
+Require Import LambdaBox_to_LambdaANF.fuel_sem.
+Require Import LambdaBox_to_LambdaANF.common.
+Require Import LambdaBox_to_LambdaANF.anf.
+Require Import LambdaBox_to_LambdaANF.anf_correct.
+Require Import LambdaBox_to_LambdaANF.anf_convert_env.
+Require Import LambdaBox_to_LambdaANF.anf_toplevel.
+Require Export LambdaANF.toplevel_theorems.
+Require Import compcert.lib.Maps.
+From Stdlib Require Import ZArith.
+Require Import Common.Common Common.compM Common.Pipeline_utils.
+From Stdlib Require Import List.
+Require Import maps_util.
+Require Import Glue.glue.
+Require Import ExtLib.Structures.Monad.
+Require Import MetaRocq.Common.BasicAst.
+From MetaRocq.Erasure Require Import EAst Erasure EWellformed.
+From MetaRocq.ErasurePlugin Require Import Erasure.
+From MetaRocq.Utils Require Import utils.
+
+From CertiRocq Require Import metarocq_pipeline pipeline.
+
+Import Monads.
+Import MonadNotation.
+Import ListNotations.
+Import common rel_comp.
+Require Import LambdaANF.term.
+
+Definition econf := Erasure.default_erasure_config.
+Import EEnvMap.
+
+From MetaRocq.Erasure Require Import EWcbvEval.
+Import EGlobalEnv.
+Import ETransform EImplementLazyForce EImplementBox.
+
+Definition env_flags :=
+  let efl := EConstructorsAsBlocks.switch_cstr_as_blocks
+    (EInlineProjections.disable_projections_env_flag 
+      (ERemoveParams.switch_no_params EWellformed.all_env_flags)) in
+  let efl' := efl_coind_to_ind efl in
+  switch_off_thunk (switch_off_box efl').
+
+(* CertiRocq does not support primitives yet *)
+Definition no_primitive_flags := {|
+  has_primint := false;
+  has_primfloat := false;
+  has_primstring := false;
+  has_primarray := false; |}.
+  
+Definition switch_off_primitives (fl : ETermFlags) :=
+{| has_tBox := fl.(has_tBox)
+  ; has_tRel := fl.(has_tRel)
+  ; has_tVar := fl.(has_tVar)
+  ; has_tEvar := fl.(has_tEvar)
+  ; has_tLambda := fl.(has_tLambda)
+  ; has_tLetIn := fl.(has_tLetIn)
+  ; has_tApp := fl.(has_tApp)
+  ; has_tConst := fl.(has_tConst)
+  ; has_tConstruct := fl.(has_tConstruct)
+  ; has_tCase := fl.(has_tCase)
+  ; has_tProj := fl.(has_tProj)
+  ; has_tFix := fl.(has_tFix)
+  ; has_tCoFix := fl.(has_tCoFix)
+  ; has_tPrim := no_primitive_flags
+  ; has_tLazy_Force := fl.(has_tLazy_Force)
+|}.
+
+(* CertiRocq's correctness lemma only supports global environments made of lambda abstractions 
+  (not arbitrary expressions or values) *)
+Lemma lambda_glob_lookup Σ :
+  lambda_glob Σ -> 
+  forall kn v, EGlobalEnv.lookup_env Σ kn = Some (ConstantDecl {| cst_body := Some v |}) -> 
+  lambda_value_pred Σ v.
+Proof.
+  induction 1.
+  - intros kn v; cbn => //.
+  - intros kn' v' hl. 
+    cbn in hl. 
+    destruct (eqb_specT kn' kn). subst kn'. noconf hl.
+    destruct d0 as [na [t ->]]. now do 2 eexists.
+    now cbn in d0.
+Qed.
+
+Lemma lambda_glob_declared Σ {efl : EEnvFlags} : 
+  wf_glob Σ ->
+  EWcbvEval.lambda_glob Σ ->
+  forall (k : kername) (decl : constant_body),
+  declared_constant Σ k decl ->
+  decl_pred (lambda_value_pred Σ) (ConstantDecl decl).
+Proof.
+  unfold EGlobalEnv.declared_constant.
+  intros hwf hv kn decl hl. destruct decl as [] => //.
+  destruct cst_body => //.
+  eapply lambda_glob_lookup in hl; tea.
+Qed.
+
+(* If the global environment is made of lambdas the all entries evaluate in 0 steps into values *)
+Lemma lambda_glob_eval_env_fuel (p : EProgram.eprogram) (efl := env_flags) :
+  wf_glob p.1 ->
+  EWcbvEval.lambda_glob p.1 ->
+  forall (k : kername) (decl : constant_body) (body : term),
+  EGlobalEnv.declared_constant p.1 k decl ->
+  cst_body decl = Some body -> exists (src_v : fuel_sem.value) (f t : nat), 
+  eval_env_fuel (Hf:=LambdaBox_resource_fuel) p.1 [] body (Val src_v) f t /\ f = <0>.
+Proof.
+  destruct p as [Σ p]; cbn; clear p.
+  intros hwf hv kn decl body hd hb.
+  have hwfd := wf.wf_glob_globals_wf _ hwf _ _ _ hd hb.
+  eapply (lambda_glob_declared _ hwf hv) in hd; tea.
+  destruct decl as [[|]]=> //. noconf hb. cbn in hd.
+  destruct hd as [na [b ->]]. do 3 eexists. split. constructor. constructor. now cbn.
+Qed.
+
+Section Correctness.
+
+  Context (func_tag kon_tag default_tag default_itag : positive).
+  Context (next_id : positive).
+
+  Notation refines_toplevel Σ ie tgm := (@refines_top default_tag default_itag tgm Σ ie).
+
+  (** To prove the correctness of connecting the MetaRocq pipeline and CertiRocq's ANF, we
+      need a stronger well-formedness property. This formalizes the remaining mismatch 
+      between metarocq's pipeline and certirocq's LambdaANF: 
+
+    - primitives are not supported in fuel_sem, and primitive arrays are forbidden in ANF conversion.
+    - the environment must be axiom free, as usual *)
+
+  Definition certirocq_flags (efl : EEnvFlags) := 
+    {| has_axioms := false; 
+       has_cstr_params := efl.(has_cstr_params); 
+       term_switches := switch_off_primitives efl.(term_switches);
+       cstr_as_blocks := efl.(cstr_as_blocks) |}.
+
+  Definition anf_convert ie tgm := 
+    convert_top_anf func_tag default_tag (M.empty _) default_itag next_id tgm []
+      (fun _ => None) ie.
+  
+  Theorem metarocq_to_anf_correct (p : EProgram.eprogram) : 
+    (* The postcondition on MetaRocq's pipeline *)
+    Transform.Transform.post (certirocq_post_metarocq_pipeline econf) p ->
+    (* Stronger invariant: no axioms, no primitives *)
+    EProgram.wf_eprogram (certirocq_flags env_flags) p ->
+    let ie := inductive_env_east (fst p) in
+    let tgm := (convert_env default_tag default_itag ie).2 in
+    forall e_tgt comp_d', 
+      anf_convert ie tgm (List.rev (fst p)) (snd p) = (compM.Ret e_tgt, comp_d') ->
+      exists M, refines_toplevel (fst p) ie tgm M (snd p) e_tgt.
+  Proof.
+    intros hp wf' ie tgm e_tgt comp_d' cvt.
+    cbn in hp.
+    match goal with
+    | [ _ : EProgram.wf_eprogram ?fl p /\ _ |- _ ] => set (efl := fl) in *
+    end.
+    destruct hp as [wfp [vg]].
+    have wf : wf_env_east ie.
+    { apply wf_env_inductive, wfp. }
+    eapply (convert_top_anf_correct func_tag kon_tag default_tag default_itag tgm (fst p) 
+      (efl:=certirocq_flags env_flags)); trea.
+    - (* The tag map is injective *) 
+      now apply convert_env_inj.
+    - (* All the original constructors are registered in the tag map *) 
+      apply convert_env_reg.
+    - (* The environment entries evaluate to values *)
+      intros kn decl hl hb hbody.
+      eapply lambda_glob_eval_env_fuel in hb; tea.
+      destruct hb as [srcv [f [t [ev eq]]]]. now exists srcv, f, t. apply wfp.
+    - (* The environment entries should evaluate to values with 0 fuel (they're lambdas) *)
+      intros kn decl b srcv f t hd hbody hev.
+      eapply lambda_glob_eval_env_fuel in hd; tea. 2:apply wfp.
+      destruct hd as [srcv' [f' [t' [ev eqf]]]].
+      eapply eval_val_exact_det in hev; tea. destruct hev as [eq [eq' eq'']].
+      now subst f' srcv' t' f.
+    - (* Wellformed declarations in the global environment *) 
+      clear wfp wf. destruct wf' as [wfΣ wf].       
+      intros kn decl body hdecl hb.
+      eapply (lookup_env_wellformed (efl := certirocq_flags (switch_off_box env_flags))) in hdecl; tea.
+      destruct decl; trivial. cbn in hdecl. cbn in hb.
+      now subst cst_body.
+    - apply wf'.
+    - (* No prims *)
+      intros s. cbn. reflexivity.
+    - eapply (cenv_tgm_coh default_tag default_itag) in wf. unfold top_cenv.
+      destruct convert_env as [[[[] ?] ?] ?]. apply wf.
+    - apply wf'.
+  Qed.
+
+  Theorem metarocq_to_anf_total (p : EProgram.eprogram) : 
+    (* The postcondition on MetaRocq's pipeline *)
+    Transform.Transform.post (certirocq_post_metarocq_pipeline econf) p ->
+    (* Stronger invariant: no axioms, no primitives *)
+    EProgram.wf_eprogram (certirocq_flags env_flags) p ->
+    let ie := inductive_env_east (fst p) in
+    let tgm := (convert_env default_tag default_itag ie).2 in
+    exists e_tgt comp_d', 
+      anf_convert ie tgm (List.rev (fst p)) (snd p) = (compM.Ret e_tgt, comp_d') /\
+      exists M, refines_toplevel (fst p) ie tgm M (snd p) e_tgt.
+  Proof.
+    intros hp wf' ie tgm.
+    match goal with
+    | [ _ : EProgram.wf_eprogram ?fl p |- _ ] => set (efl := fl) in *
+    end.
+    destruct hp as [wfp [vg]].
+    have wf : wf_env_east ie.
+    { apply wf_env_inductive. apply wf'. }
+    unshelve eset (prf := anf_corresp.convert_top_anf_total func_tag default_tag default_itag tgm (fst p) 
+      (efl:=certirocq_flags env_flags) eq_refl (M.empty _) [] (proj1 wf') eq_refl eq_refl eq_refl eq_refl eq_refl eq_refl
+      _
+      (convert_env_reg _ _ _) next_id ie _ (proj2 wf')); trea.
+    destruct prf as [e_tgt [comp_d' heq]]. exists e_tgt, comp_d'. split.
+    unfold anf_convert. exact heq.
+    eapply metarocq_to_anf_correct; tea. split => //.
+  Qed.
+  
+  (*
+  Lemma metarocq_anf_pipeline (p : EProgram.eprogram) opts : 
+    (* The postcondition on MetaRocq's pipeline *)
+    Transform.Transform.post (certirocq_post_metarocq_pipeline econf) p ->
+    (* Stronger invariant: no axioms, no primitives *)
+    EProgram.wf_eprogram (certirocq_flags env_flags) p ->
+    let ie := inductive_env_east (fst p) in
+    let tgm := (convert_env default_tag default_itag ie).2 in
+    let cenv := (convert_env default_tag default_itag ie).1.1.1.2 in
+    exists e_tgt comp_d', 
+      anf_convert ie tgm (List.rev (fst p)) (snd p) = (compM.Ret e_tgt, comp_d') /\
+      exists e_tgt' data, 
+        anf_pipeline next_id opts e_tgt comp_d' = (compM.Ret e_tgt', data) /\
+        forall (v_src : fuel_sem.value) (f_src t_src : nat),
+        eval_env_fuel (Hf := LambdaBox_resource_fuel) (Ht := LambdaBox_resource_trace) p.1 [] p.2 (Val v_src) f_src t_src ->
+        exists (v2 : val) (c2 : nat) (t2 : nat × nat), eval.bstep_fuel  cenv emp e_tgt' c2 (eval.Res v2) t2 /\ anf_toplevel.value_ref tgm v_src v2.
+         (* /\ refines (trace:=nat * nat) cenv value_ref_cc e_tgt e_tgt'. *)
+  Proof.
+    intros hp wf' ie tgm cenv.
+    destruct (metarocq_to_anf_total p hp wf') as [e_tgt [comp_d' [heq [M href]]]].
+    exists e_tgt, comp_d'. split => //.
+    pose proof (anf_pipeline_whole_program_correct cenv next_id opts e_tgt comp_d').
+    forward H.
+    { admit. }
+    forward H.
+    { admit. }
+    forward H by admit.
+    destruct H as [e' [c' [hanf href']]].
+    exists e', c'. split => //.
+    do 2 red in href.
+    intros v_src f_src t_src hev.
+    specialize (href v_src f_src t_src hev) as [v_tgt [ctgt [hev' [hc href]]]].
+    set (top_cenv := top_cenv _ _ _) in hev'. 
+    assert (top_cenv = cenv). unfold top_cenv, cenv. unfold anf_toplevel.top_cenv. destruct convert_env as [[[[] ?] ?] ?]. reflexivity.
+    clearbody top_cenv. subst top_cenv.
+    destruct href' as [href' _].    
+    specialize (href' v_tgt _ _ hev'). (href' v_tgt ctgt hev') as [v2 [c2 [t2 [hev'' href'']]]].
+    destruct (href v_src f_src t_src hev).
+    exists v2, c2, t2
+
+    red in href'.
+    exists M. split => //.
+    Print anf_toplevel.refines.
+    Print refines.
+  Admitted.
+*)
+
+    
+
+
+
+
+(* 
+  Theorem metarocq_to_anf_eval (p : EProgram.eprogram) : 
+    (* The postcondition on MetaRocq's pipeline *)
+    Transform.Transform.post (certirocq_post_metarocq_pipeline econf) p ->
+    (* Stronger invariant: no axioms, no primitives *)
+    EProgram.wf_eprogram (certirocq_flags env_flags) p ->
+    let ie := inductive_env_east (fst p) in
+    let tgm := (convert_env default_tag default_itag ie).2 in
+    forall v_src, 
+      eval (fst p) (snd p) v_src ->
+      exists M e_tgt v_tgt c_tgt,
+      anf_convert ie tgm (List.rev (fst p)) (snd p) = (compM.Ret e_tgt, comp_d') /\
+      eval.bstep_fuel (cenv comp_d') (M.empty val) e_tgt c_tgt (eval.Res v_tgt) tt /\
+      anf_toplevel.value_ref tgm v_src v_tgt. *)
+      
+End Correctness.
